lab-3 done!!!!
lets goooooo

lab3 testing dbg ver/Lab3_circular_buffer_template.dfy
@@ -6,8 +6,9 @@ class CircularMemory
   var read_position : int;
   var write_position : int;
   var isFlipped : bool;
+  var cap : int;
 
-  constructor Init(cap : int) 
+  constructor Init(cap : int)
     requires cap > 0
   {
     cells := new int[cap];
@@ -18,11 +19,11 @@ class CircularMemory
   predicate Valid() 
     reads this
   {
-    cells.Length > 0 && 
-    read_position >= 0 && 
-    read_position < cells.Length 
-    && write_position >= 0 
-    && write_position < cells.Length
+    cap == cells.Length && write_position >= 0
+    && write_position < cap
+    && read_position >= 0 && read_position < cap
+    && ((!isFlipped <==> read_position<= write_position)
+    || (isFlipped <==> read_position >= write_position))
   }
 
   predicate isFull()
@@ -40,34 +41,130 @@ class CircularMemory
    method Read() returns (isSuccess : bool, content : int)
     modifies this 
     requires Valid()
-    ensures  Valid()
-    ensures  isSuccess ==> old(cells) == cells 
-                           && ((old(read_position) == read_position-1)  
-                           || (old(read_position) == cells.Length-1 
-                           && read_position == 0 && !isFlipped))
-                           && old(write_position) == write_position
+    ensures Valid()
+    ensures  isSuccess ==> old(cells) == cells && 
+    ((old(read_position) == read_position-1) || (old(read_position) == cells.Length-1 && read_position == 0 && !isFlipped)) 
+    && old(write_position) == write_position
     ensures !isSuccess ==> (isEmpty() && old(cells) == cells)
 
   {
-    if(isFlipped){
-        content := cells[read_position];
-        isSuccess := true; 
-        if (read_position == cells.Length-1){ read_position := 0; isFlipped := false;}
-        else {read_position := read_position+1;}
+    if (isFlipped){
+      //read = write
+      if(read_position == write_position){
+
+        //if we are on last index
+        if (read_position < cells.Length-1){
+          content := cells[read_position];
+          read_position := read_position+1;
+          isSuccess := true;
+        }
+
+        //if we are on last index
+        else {
+          content := cells[read_position];
+          read_position := 0;
+          isSuccess := true;
+          isFlipped := false;
+        }
+      }
+      // read > write
+      else{
+
+        //read == cells.Length-1
+        if  (read_position == cells.Length-1){
+          content := cells[read_position];
+          read_position := 0;
+          isSuccess := true;
+          isFlipped := false;
+        }
+
+        //read < cells.Length-1
+        else {
+          content := cells[read_position];
+          read_position := read_position+1;
+          isSuccess := true;
+        }
+      }
     }
+    //if not flipped
     else{
-      // if Empty
+      //if read = write
       if (read_position == write_position){
         content := 0;
         isSuccess := false;
       }
-      // if read_position < write_position
+      //if read < write
       else {
         content := cells[read_position];
-        read_position := read_position+1;
         isSuccess := true;
+        read_position := read_position + 1;
+      }
+    }
+    }
+    method Write(input : int) returns (isSuccess : bool)
+      modifies this, this.cells
+      requires Valid()
+      ensures  Valid()
+      ensures  isSuccess ==> ((old(write_position) == write_position-1 || ((old(write_position) == cells.Length-1) && (write_position == 0) && (isFlipped)))
+      && (old(read_position) == read_position))
+      ensures !isSuccess ==> (old(cells) == cells && isFull())
+  {
+    if (isFlipped) {
+
+      // write = read AKA full
+      if (read_position == write_position) {
+        isSuccess := false;
+      }
+
+      // write < read
+      else {
+        cells[write_position] := input;
+        isSuccess := true;
+        write_position := write_position + 1;
+      }
+    }
+    // if not flipped
+    else {
+      
+      // if write = read
+      if (write_position == read_position){
+          cells[write_position] := input;
+          isSuccess := true;
+
+  
+        // if write = cells.Length-1
+        if (write_position == cells.Length-1){
+          isFlipped := true;
+          write_position := 0;
+        }
+
+        // if write < cells.Length-1
+        else{
+          write_position := write_position+1;
+        }
+      }
+
+      // if write > read
+      else{
+        cells[write_position] := input;
+        isSuccess := true;
+        
+        // if write == cells.Length-1
+        if(write_position == cells.Length-1){
+          isFlipped := true;
+          write_position := 0;
+        }
+
+        // if write < cells.Length-1
+        else{
+          write_position := write_position + 1;
+        }
       }
 
     }
+    
   }
-}
+
+
+  }
+ 
